nola/examples/logic/subst.v
@@ -49,7 +49,6 @@ Local Fixpoint nsubstlg {κ Γ Γᵍ V} (Φ : nPred V) (P : nProp κ Γ)
   | n_0 c => λ _, n_0 c | n_l0 c => λ _, n_l0 c
   | n_1 c P => λ eq, n_1 c (nsubstlg Φ P eq)
   | n_2 c P Q => λ eq, n_2 c (nsubstlg Φ P eq) (nsubstlg Φ Q eq)
-  | n_l1 c P => λ eq, n_l1 c (nsubstlg Φ P eq)
   | n_cwpw c W Ψ => λ eq, n_cwpw c (nsubstlg Φ W eq) (λ v, nsubstlg Φ (Ψ v) eq)
   | n_g1 c P => λ eq, n_g1 c (nsubstlg Φ P (eq_app_assoc_d eq))
   | n_g1f c Ψ => λ eq, n_g1f c (λ q, nsubstlg Φ (Ψ q) (eq_app_assoc_d eq))
@@ -100,7 +99,6 @@ Fixpoint nsubstlu {κ Γ Γᵘ V} (Φ : nPred V) (P : nProp κ Γ)
   match P with
   | n_0 c => λ _ _, n_0 c | n_l0 c => λ _ _, n_l0 c
   | n_1 c P => λ eq gn, n_1 c (nsubstlu Φ P eq gn)
-  | n_l1 c P => λ eq gn, n_l1 c (nsubstlu Φ P eq gn)
   | n_2 c P Q => λ eq gn, n_2 c (nsubstlu Φ P eq gn) (nsubstlu Φ Q eq gn)
   | n_cwpw c W Ψ => λ eq gn,
       n_cwpw c (nsubstlu Φ W eq gn) (λ v, nsubstlu Φ (Ψ v) eq gn)
@@ -155,7 +153,6 @@ Fixpoint nhgt {κ Γ} (P : nProp κ Γ) : hgt :=
   match P with
   | n_0 _ | n_l0 _ | n_g1 _ _ | n_g1f _ _ | ¢ᵍ _ | %ᵍˢ _ | %ᵍˡ _ | %ᵘˢ _
     | !ᵘˢ _ => Hgt₀
-  | n_l1 _ P => Hgt₁ (nhgt P)
   | ¢ᵘ P => nhgt P | n_1 _ P | ∀: _, P | ∃: _, P => Hgt₁ (nhgt P)
   | n_2 _ P Q => Hgt₂ (nhgt P) (nhgt Q) | ∀' Φ | ∃' Φ => Hgtᶠ (λ a, nhgt (Φ a))
   | n_cwpw _ W Φ => Hgt₂ (nhgt W) (Hgtᶠ (λ a, nhgt (Φ a)))
